theories/Reflection2/PredMonadState.v
@@ -1,0 +1,42 @@
+Require Export PredMonad.Reflection2.PredMonad.
+Require Export PredMonad.Reflection2.MonadState.
+
+
+(***
+ *** Predicate Monads with State Effects
+ ***)
+
+Class PredMonadState M PM St {OM: OTypeF1 M} {OPM: OTypeF1 PM} {OSt: OType St}
+      {MOps: @MonadOps M OM} {PMOps: @MonadOps PM OPM}
+      {PredOps: @PredMonadOps M PM OM OPM}
+      {MSOps: @MonadStateOps M OM St OSt} {PMSOps: @MonadStateOps PM OPM St OSt}
+  : Prop :=
+  {
+    (* M and PM must form a predicate monad *)
+    predmonadstate_predmonad :> PredMonad M PM;
+
+    (* Lifting for getM and putM *)
+    predmonadstate_liftP_getM : liftP @o@ getM =o= getM;
+    predmonadstate_liftP_putM :
+      forall s, liftP @o@ (putM @o@ s) =o= putM @o@ s;
+
+    (* FIXME HERE: laws for commuting forallP and existsP with getM and putM *)
+  }.
+
+
+(***
+ *** Hoare Logic using Predicate Monads
+ ***)
+
+Definition HoareP `{PredMonadState} `{OType} :
+  (St -o> Flip Prop) -o> (St -o> A -o> St -o> Prop) -o> PM A _ :=
+  ofun pre =>
+  ofun post =>
+  do s_pre <- getM;
+    assumingP
+      @o@ (pre @o@ s_pre)
+      @o@ (do x <- trueP;
+             do s_post <- getM;
+             do unused
+                <- assertP @o@ (post @o@ s_pre @o@ x @o@ s_post);
+             returnM @o@ x).
